Wrote up stack conversion

04Stack/StackConversion.thy
@@ -2,119 +2,95 @@ theory StackConversion
   imports Stack
 begin
 
-fun unwind' :: "frame\<^sub>k list \<Rightarrow> expr\<^sub>d \<Rightarrow> expr\<^sub>d" where
-  "unwind' [] e = e"
-| "unwind' (FApp1\<^sub>k e\<^sub>2 # s) e = unwind' s (App\<^sub>d e e\<^sub>2)"
-| "unwind' (FApp2\<^sub>k e\<^sub>1 # s) e = unwind' s (App\<^sub>d e\<^sub>1 e)"
-| "unwind' (FReturn\<^sub>k # s) e = unwind' s e"
+subsection \<open>Stack conversion\<close>
 
-primrec unwind :: "state\<^sub>k \<Rightarrow> expr\<^sub>d" where
-  "unwind (S\<^sub>k b s e) = unwind' s e"
+text \<open>Now we define stack conversion. There is no good way to define it in a forward direction, 
+since most expressions have more than one possible equivalent stack state, and even picking one 
+arbitrarily - the one with an empty stack, say - would fail because the stack evaluation relation 
+only has an empty stack at the very beginning and end of evaluation. Instead, we define it 
+backwards, which is simple to write, but will give us trouble with our reconstruction lemmas later.\<close>
 
-lemma [simp]: "s :\<^sub>k t' \<rightarrow> t \<Longrightarrow> [] \<turnstile>\<^sub>d e : t' \<Longrightarrow> [] \<turnstile>\<^sub>d unwind' s e : t"
+fun unstack' :: "frame\<^sub>k list \<Rightarrow> expr\<^sub>d \<Rightarrow> expr\<^sub>d" where
+  "unstack' [] e = e"
+| "unstack' (FApp1\<^sub>k e\<^sub>2 # s) e = unstack' s (App\<^sub>d e e\<^sub>2)"
+| "unstack' (FApp2\<^sub>k e\<^sub>1 # s) e = unstack' s (App\<^sub>d e\<^sub>1 e)"
+| "unstack' (FReturn\<^sub>k # s) e = unstack' s e"
+
+lemma typesafe\<^sub>k' [simp]: "s :\<^sub>k t' \<rightarrow> t \<Longrightarrow> [] \<turnstile>\<^sub>d e : t' \<Longrightarrow> [] \<turnstile>\<^sub>d unstack' s e : t"
   by (induction s t' t arbitrary: e rule: typing_stack\<^sub>k.induct) simp_all
 
-theorem typesafed [simp]: "\<Sigma> :\<^sub>k t \<Longrightarrow> [] \<turnstile>\<^sub>d unwind \<Sigma> : t"
-  by (induction \<Sigma> t rule: typing_state\<^sub>k.induct) simp_all
-
-lemma [simp]: "s :\<^sub>k t' \<rightarrow> t \<Longrightarrow> e \<leadsto>\<^sub>d e' \<Longrightarrow> unwind' s e \<leadsto>\<^sub>d unwind' s e'"
+lemma unstack'_eval [simp]: "s :\<^sub>k t' \<rightarrow> t \<Longrightarrow> e \<leadsto>\<^sub>d e' \<Longrightarrow> unstack' s e \<leadsto>\<^sub>d unstack' s e'"
   by (induction s t' t arbitrary: e e' rule: typing_stack\<^sub>k.induct) simp_all
 
-theorem correctd: "\<Sigma> \<leadsto>\<^sub>k \<Sigma>' \<Longrightarrow> \<Sigma> :\<^sub>k t \<Longrightarrow> iter (\<leadsto>\<^sub>d) (unwind \<Sigma>) (unwind \<Sigma>')"
-proof (induction \<Sigma> \<Sigma>' rule: eval\<^sub>k.induct)
+text \<open>Converting a full state is also simple. Once we have that, typesafety and completeness follow 
+immediately. Note the use of \<open>iter\<close> in the completeness theorem. Actually, it will only ever be zero 
+or one \<open>\<leadsto>\<^sub>d\<close> steps for each \<open>\<leadsto>\<^sub>k\<close> step, since the redex-search steps don't change the unstacked 
+expression, and reduction steps are equivalent to a single evaluation step; but as mentioned when we 
+defined \<open>iter\<close>, we reuse it for this sort of "zero or one" relation as well.\<close>
+
+primrec unstack :: "state\<^sub>k \<Rightarrow> expr\<^sub>d" where
+  "unstack (S\<^sub>k b s e) = unstack' s e"
+
+theorem typesafe\<^sub>k [simp]: "\<Sigma>\<^sub>k :\<^sub>k t \<Longrightarrow> [] \<turnstile>\<^sub>d unstack \<Sigma>\<^sub>k : t"
+  by (induction \<Sigma>\<^sub>k t rule: typing_state\<^sub>k.induct) simp_all
+
+theorem complete\<^sub>k: "\<Sigma>\<^sub>k \<leadsto>\<^sub>k \<Sigma>\<^sub>k' \<Longrightarrow> \<Sigma>\<^sub>k :\<^sub>k t \<Longrightarrow> iter (\<leadsto>\<^sub>d) (unstack \<Sigma>\<^sub>k) (unstack \<Sigma>\<^sub>k')"
+proof (induction \<Sigma>\<^sub>k \<Sigma>\<^sub>k' rule: eval\<^sub>k.induct)
   case (ev\<^sub>k_app3 t\<^sub>1 e\<^sub>1 s e\<^sub>2)
   then obtain t\<^sub>2 where "(s :\<^sub>k t\<^sub>2 \<rightarrow> t) \<and> value\<^sub>d e\<^sub>2" by blast
   moreover hence "App\<^sub>d (Lam\<^sub>d t\<^sub>1 e\<^sub>1) e\<^sub>2 \<leadsto>\<^sub>d subst\<^sub>d 0 e\<^sub>2 e\<^sub>1" by simp
-  ultimately have "unwind' s (App\<^sub>d (Lam\<^sub>d t\<^sub>1 e\<^sub>1) e\<^sub>2) \<leadsto>\<^sub>d unwind' s (subst\<^sub>d 0 e\<^sub>2 e\<^sub>1)" by auto
+  ultimately have "unstack' s (App\<^sub>d (Lam\<^sub>d t\<^sub>1 e\<^sub>1) e\<^sub>2) \<leadsto>\<^sub>d unstack' s (subst\<^sub>d 0 e\<^sub>2 e\<^sub>1)" by auto
   thus ?case by simp
 qed simp_all
 
+text \<open>Correctness is another matter. There are a few problems here, and the biggest of them is 
+\<open>FReturn\<^sub>k\<close>. A state which unstacks to a given expression might have any number of return frames in 
+its stack, anywhere. We define a function to help deal with these empty frames.\<close>
+
 primrec all_returns :: "frame\<^sub>k list \<Rightarrow> bool" where
   "all_returns [] = True"
-| "all_returns (r # rs) = (r = FReturn\<^sub>k \<and> all_returns rs)"
+| "all_returns (f # s) = (f = FReturn\<^sub>k \<and> all_returns s)"
 
-lemma unwind_returns [elim]: "all_returns sr \<Longrightarrow> unwind' sr e = e"
-  by (induction sr) (simp_all add: all_returns_def)
+lemma unstack_returns [elim]: "all_returns s \<Longrightarrow> unstack' s e = e"
+  by (induction s) (simp_all add: all_returns_def)
 
-lemma [dest]: "FApp1\<^sub>k e # sr :\<^sub>k t' \<rightarrow> t \<Longrightarrow> all_returns sr \<Longrightarrow> 
+lemma fapp1_and_returns [dest]: "FApp1\<^sub>k e # s :\<^sub>k t' \<rightarrow> t \<Longrightarrow> all_returns s \<Longrightarrow> 
     (\<And>t\<^sub>1. t' = Arrow t\<^sub>1 t \<Longrightarrow> [] \<turnstile>\<^sub>d e : t\<^sub>1 \<Longrightarrow> P) \<Longrightarrow> P"
-  by (induction sr) fastforce+
+  by (induction s) fastforce+
 
-lemma [dest]: "FApp2\<^sub>k e # sr :\<^sub>k t' \<rightarrow> t \<Longrightarrow> all_returns sr \<Longrightarrow> 
+lemma fapp2_and_returns [dest]: "FApp2\<^sub>k e # sr :\<^sub>k t' \<rightarrow> t \<Longrightarrow> all_returns sr \<Longrightarrow> 
     ([] \<turnstile>\<^sub>d e : Arrow t' t \<Longrightarrow> value\<^sub>d e \<Longrightarrow> P) \<Longrightarrow> P"
   by (induction sr) fastforce+
 
-lemma [dest]: "sr @ s :\<^sub>k t' \<rightarrow> t \<Longrightarrow> all_returns sr \<Longrightarrow> (s :\<^sub>k t' \<rightarrow> t \<Longrightarrow> P) \<Longrightarrow> P"
-  by (induction sr) fastforce+
+lemma returns_prepended [dest]: "s @ s' :\<^sub>k t' \<rightarrow> t \<Longrightarrow> all_returns s \<Longrightarrow> (s' :\<^sub>k t' \<rightarrow> t \<Longrightarrow> P) \<Longrightarrow> P"
+  by (induction s) fastforce+
 
-lemma [dest]: "App\<^sub>d e\<^sub>1 e\<^sub>2 = unwind' s e \<Longrightarrow> (all_returns s \<and> e = App\<^sub>d e\<^sub>1 e\<^sub>2) \<or> 
-  (\<exists>s' sr. all_returns sr \<and> ((s = s' @ FApp1\<^sub>k e\<^sub>2 # sr \<and> e\<^sub>1 = unwind' s' e) \<or> 
-    (s = s' @ FApp2\<^sub>k e\<^sub>1 # sr \<and> e\<^sub>2 = unwind' s' e)))"
-proof (induction s e rule: unwind'.induct)
-  case (2 e\<^sub>2' s e)
-  thus ?case
-  proof (cases "all_returns s \<and> App\<^sub>d e e\<^sub>2' = App\<^sub>d e\<^sub>1 e\<^sub>2")
-    case False
-    with 2 obtain s' sr where S: "all_returns sr \<and> ((s = s' @ FApp1\<^sub>k e\<^sub>2 # sr \<and> 
-      e\<^sub>1 = unwind' s' (App\<^sub>d e e\<^sub>2')) \<or> (s = s' @ FApp2\<^sub>k e\<^sub>1 # sr \<and> e\<^sub>2 = unwind' s' (App\<^sub>d e e\<^sub>2')))" 
-        by fastforce
-    thus ?thesis
-    proof (cases "s = s' @ FApp1\<^sub>k e\<^sub>2 # sr \<and> e\<^sub>1 = unwind' s' (App\<^sub>d e e\<^sub>2')")
-      case False
-      with S have "all_returns sr \<and> s = s' @ FApp2\<^sub>k e\<^sub>1 # sr \<and> e\<^sub>2 = unwind' s' (App\<^sub>d e e\<^sub>2')" by simp
-      moreover hence "FApp1\<^sub>k e\<^sub>2' # s' @ FApp2\<^sub>k e\<^sub>1 # sr = (FApp1\<^sub>k e\<^sub>2' # s') @ FApp2\<^sub>k e\<^sub>1 # sr \<and> 
-        unwind' s' (App\<^sub>d e e\<^sub>2') = unwind' (FApp1\<^sub>k e\<^sub>2' # s') e" by simp
-      ultimately show ?thesis by blast
-    qed fastforce+
-  qed fastforce+
-next
-  case (3 e\<^sub>1' s e)
-  thus ?case
-  proof (cases "all_returns s \<and> App\<^sub>d e\<^sub>1' e = App\<^sub>d e\<^sub>1 e\<^sub>2")
-    case False
-    with 3 obtain s' sr where S: "all_returns sr \<and> ((s = s' @ FApp1\<^sub>k e\<^sub>2 # sr \<and> 
-      e\<^sub>1 = unwind' s' (App\<^sub>d e\<^sub>1' e)) \<or> (s = s' @ FApp2\<^sub>k e\<^sub>1 # sr \<and> e\<^sub>2 = unwind' s' (App\<^sub>d e\<^sub>1' e)))" 
-        by fastforce
-    thus ?thesis
-    proof (cases "s = s' @ FApp1\<^sub>k e\<^sub>2 # sr \<and> e\<^sub>1 = unwind' s' (App\<^sub>d e\<^sub>1' e)")
-      case False
-      with S have "all_returns sr \<and> s = s' @ FApp2\<^sub>k e\<^sub>1 # sr \<and> e\<^sub>2 = unwind' s' (App\<^sub>d e\<^sub>1' e)" by simp
-      moreover hence "FApp2\<^sub>k e\<^sub>1' # s' @ FApp2\<^sub>k e\<^sub>1 # sr = (FApp2\<^sub>k e\<^sub>1' # s') @ FApp2\<^sub>k e\<^sub>1 # sr \<and> 
-        e\<^sub>2 = unwind' (FApp2\<^sub>k e\<^sub>1' # s') e" by simp
-      ultimately show ?thesis by blast
-    qed fastforce+
-  qed fastforce+
-next
-  case (4 s e)
-  thus ?case
-  proof (cases "all_returns s \<and> e = App\<^sub>d e\<^sub>1 e\<^sub>2")
-    case False
-    with 4 obtain s' sr where S: "all_returns sr \<and> ((s = s' @ FApp1\<^sub>k e\<^sub>2 # sr \<and> e\<^sub>1 = unwind' s' e) \<or> 
-      (s = s' @ FApp2\<^sub>k e\<^sub>1 # sr \<and> e\<^sub>2 = unwind' s' e))" by fastforce
-    thus ?thesis
-    proof (cases "s = s' @ FApp1\<^sub>k e\<^sub>2 # sr \<and> e\<^sub>1 = unwind' s' e")
-      case False
-      with S have "all_returns sr \<and> s = s' @ FApp2\<^sub>k e\<^sub>1 # sr \<and> e\<^sub>2 = unwind' s' e" by simp
-      moreover hence "FReturn\<^sub>k # s' @ FApp2\<^sub>k e\<^sub>1 # sr = (FReturn\<^sub>k # s') @ FApp2\<^sub>k e\<^sub>1 # sr \<and> 
-        e\<^sub>2 = unwind' (FReturn\<^sub>k # s') e" by simp
-      ultimately show ?thesis by blast
-    qed fastforce+
-  qed fastforce+
-qed simp_all
+lemma unstack_to_value' [simp]: "value\<^sub>d v \<Longrightarrow> v = unstack' s e \<Longrightarrow> all_returns s \<and> e = v"
+  by (induction s e rule: unstack'.induct) simp_all
 
-lemma [simp]: "value\<^sub>d v \<Longrightarrow> v = unwind' s e \<Longrightarrow> all_returns s \<and> e = v"
-  by (induction s e rule: unwind'.induct) simp_all
+lemma unstack_to_value [simp]: "value\<^sub>d v \<Longrightarrow> v = unstack \<Sigma>\<^sub>k \<Longrightarrow> \<exists>b s. \<Sigma>\<^sub>k = S\<^sub>k b s v \<and> all_returns s"
+  by (induction \<Sigma>\<^sub>k) simp_all
 
-lemma [simp]: "value\<^sub>d v \<Longrightarrow> v = unwind \<Sigma> \<Longrightarrow> \<exists>b s. \<Sigma> = S\<^sub>k b s v \<and> all_returns s"
-  by (induction \<Sigma>) simp_all
+text \<open>Now we prove our reconstruction lemma for \<open>App\<^sub>d\<close>s. Without returns, this would be much simpler 
+- but as mentioned, we need them for the next stage.\<close>
 
-lemma [simp]: "all_returns sr \<Longrightarrow> unwind' (s @ FApp1\<^sub>k e\<^sub>2 # sr) e = App\<^sub>d (unwind' s e) e\<^sub>2"
-  by (induction s e rule: unwind'.induct) auto
+lemma unstack_to_app [consumes 1, case_names Empty FApp1\<^sub>k FApp2\<^sub>k]: "App\<^sub>d e\<^sub>1 e\<^sub>2 = unstack' s e \<Longrightarrow> 
+    (all_returns s \<Longrightarrow> e = App\<^sub>d e\<^sub>1 e\<^sub>2 \<Longrightarrow> P) \<Longrightarrow> 
+    (\<And>s' sr. all_returns sr \<Longrightarrow> s = s' @ FApp1\<^sub>k e\<^sub>2 # sr \<Longrightarrow> e\<^sub>1 = unstack' s' e \<Longrightarrow> P) \<Longrightarrow>
+    (\<And>s' sr. all_returns sr \<Longrightarrow> s = s' @ FApp2\<^sub>k e\<^sub>1 # sr \<Longrightarrow> e\<^sub>2 = unstack' s' e \<Longrightarrow> P) \<Longrightarrow> 
+    P"
+  by (induction s e rule: unstack'.induct) fastforce+
 
-lemma [simp]: "all_returns sr \<Longrightarrow> unwind' (s @ FApp2\<^sub>k e\<^sub>1 # sr) e = App\<^sub>d e\<^sub>1 (unwind' s e)"
-  by (induction s e rule: unwind'.induct) auto
+lemma unstack_from_app1 [simp]: "all_returns sr \<Longrightarrow> 
+    unstack' (s @ FApp1\<^sub>k e\<^sub>2 # sr) e = App\<^sub>d (unstack' s e) e\<^sub>2"
+  by (induction s e rule: unstack'.induct) auto
 
-lemma eval_returns [simp]: "all_returns sr \<Longrightarrow> value\<^sub>d v \<Longrightarrow> iter (\<leadsto>\<^sub>k) (S\<^sub>k b (sr @ s) v) (S\<^sub>k True s v)"
+lemma unstack_from_app2 [simp]: "all_returns sr \<Longrightarrow> 
+    unstack' (s @ FApp2\<^sub>k e\<^sub>1 # sr) e = App\<^sub>d e\<^sub>1 (unstack' s e)"
+  by (induction s e rule: unstack'.induct) auto
+
+lemma eval_returns_in_front [simp]: "all_returns sr \<Longrightarrow> value\<^sub>d v \<Longrightarrow> 
+  iter (\<leadsto>\<^sub>k) (S\<^sub>k b (sr @ s) v) (S\<^sub>k True s v)"
 proof (induction sr arbitrary: b)
   case (Cons a sr)
   hence "iter (\<leadsto>\<^sub>k) (S\<^sub>k b (FReturn\<^sub>k # sr @ s) v) (S\<^sub>k True (FReturn\<^sub>k # sr @ s) v)" by simp
@@ -124,55 +100,51 @@ proof (induction sr arbitrary: b)
   with Cons show ?case by simp
 qed simp_all
 
-lemma [simp]: "unwind' s e \<leadsto>\<^sub>d e' \<Longrightarrow> s :\<^sub>k t' \<rightarrow> t \<Longrightarrow> [] \<turnstile>\<^sub>d e : tt \<Longrightarrow> (b \<Longrightarrow> value\<^sub>d e) \<Longrightarrow>
-  \<exists>b' s' e''. iter (\<leadsto>\<^sub>k) (S\<^sub>k b s e) (S\<^sub>k b' s' e'') \<and> e' = unwind' s' e''"
-proof (induction "unwind' s e" e' arbitrary: b s e t tt rule: eval\<^sub>d.induct)
+text \<open>And finally, the main lemma for correctness. Being able to reconstruct the stack state that 
+was unstacked to an \<open>App\<^sub>d\<close> is crucial to make this work.\<close>
+
+lemma correctness\<^sub>k' [simp]: "unstack' s e \<leadsto>\<^sub>d e' \<Longrightarrow> s :\<^sub>k t' \<rightarrow> t \<Longrightarrow> [] \<turnstile>\<^sub>d e : tt \<Longrightarrow> 
+  b \<longrightarrow> value\<^sub>d e \<Longrightarrow> \<exists>b' s' e''. iter (\<leadsto>\<^sub>k) (S\<^sub>k b s e) (S\<^sub>k b' s' e'') \<and> e' = unstack' s' e''"
+proof (induction "unstack' s e" e' arbitrary: b s e t tt rule: eval\<^sub>d.induct)
   case (ev\<^sub>d_app1 e\<^sub>1 e\<^sub>1' e\<^sub>2)
-  thus ?case
-  proof (cases "all_returns s \<and> e = App\<^sub>d e\<^sub>1 e\<^sub>2")
-    case True
+  from ev\<^sub>d_app1(3) show ?case
+  proof (induction rule: unstack_to_app)
+    case Empty
     with ev\<^sub>d_app1 have B: "\<not>b" by (cases b) simp_all
-    from ev\<^sub>d_app1 True obtain t\<^sub>1 where T1: "([] \<turnstile>\<^sub>d e\<^sub>1 : Arrow t\<^sub>1 tt) \<and> ([] \<turnstile>\<^sub>d e\<^sub>2 : t\<^sub>1)" by blast
+    from ev\<^sub>d_app1 Empty obtain t\<^sub>1 where T1: "([] \<turnstile>\<^sub>d e\<^sub>1 : Arrow t\<^sub>1 tt) \<and> ([] \<turnstile>\<^sub>d e\<^sub>2 : t\<^sub>1)" by blast
     have "[] :\<^sub>k t' \<rightarrow> t'" by simp
     with ev\<^sub>d_app1 B T1 obtain b' s' e'' where E: "iter (\<leadsto>\<^sub>k) (S\<^sub>k False [] e\<^sub>1) (S\<^sub>k b' s' e'') \<and> 
-      e\<^sub>1' = unwind' s' e''" by fastforce
+      e\<^sub>1' = unstack' s' e''" by fastforce
     hence "iter (\<leadsto>\<^sub>k) (S\<^sub>k False ([] @ FApp1\<^sub>k e\<^sub>2 # s) e\<^sub>1) (S\<^sub>k b' (s' @ FApp1\<^sub>k e\<^sub>2 # s) e'')" 
       by (metis eval\<^sub>k_under_iter)
     hence "iter (\<leadsto>\<^sub>k) (S\<^sub>k False (FApp1\<^sub>k e\<^sub>2 # s) e\<^sub>1) (S\<^sub>k b' (s' @ FApp1\<^sub>k e\<^sub>2 # s) e'')" by simp
     hence "iter (\<leadsto>\<^sub>k) (S\<^sub>k False s (App\<^sub>d e\<^sub>1 e\<^sub>2)) (S\<^sub>k b' (s' @ FApp1\<^sub>k e\<^sub>2 # s) e'')" 
       by (metis ev\<^sub>k_app1 iter_step)
-    with True B E show ?thesis by fastforce
+    with Empty B E show ?thesis by fastforce
   next
-    case False
-    with ev\<^sub>d_app1 obtain s' sr where S: "all_returns sr \<and> 
-      ((s = s' @ FApp1\<^sub>k e\<^sub>2 # sr \<and> e\<^sub>1 = unwind' s' e) \<or> 
-        (s = s' @ FApp2\<^sub>k e\<^sub>1 # sr \<and> e\<^sub>2 = unwind' s' e))" by fast
-    thus ?thesis
-    proof (cases "s = s' @ FApp1\<^sub>k e\<^sub>2 # sr \<and> e\<^sub>1 = unwind' s' e")
-      case True
-      with ev\<^sub>d_app1 obtain t'' where "(s' :\<^sub>k t' \<rightarrow> t'') \<and> (FApp1\<^sub>k e\<^sub>2 # sr :\<^sub>k t'' \<rightarrow> t)" by fastforce
-      with ev\<^sub>d_app1 True obtain b' ss' e'' where S': "iter (\<leadsto>\<^sub>k) (S\<^sub>k b s' e) (S\<^sub>k b' ss' e'') \<and> 
-        e\<^sub>1' = unwind' ss' e''" by blast
-      hence X: "iter (\<leadsto>\<^sub>k) (S\<^sub>k b (s' @ FApp1\<^sub>k e\<^sub>2 # sr) e) (S\<^sub>k b' (ss' @ FApp1\<^sub>k e\<^sub>2 # sr) e'')" by simp
-      from S S' have "App\<^sub>d e\<^sub>1' e\<^sub>2 = unwind' (ss' @ FApp1\<^sub>k e\<^sub>2 # sr) e''" by simp
-      with True X show ?thesis by blast
-    next
-      case False
-      with S have "s = s' @ FApp2\<^sub>k e\<^sub>1 # sr \<and> e\<^sub>2 = unwind' s' e" by simp
-      with ev\<^sub>d_app1 obtain t\<^sub>1 where "(s' :\<^sub>k t' \<rightarrow> t\<^sub>1) \<and> (FApp2\<^sub>k e\<^sub>1 # sr :\<^sub>k t\<^sub>1 \<rightarrow> t)" by fastforce
-      with S have "([] \<turnstile>\<^sub>d e\<^sub>1 : Arrow t\<^sub>1 t) \<and> value\<^sub>d e\<^sub>1" by fastforce
-      with ev\<^sub>d_app1 show ?thesis by (metis val_no_eval\<^sub>d)
-    qed
+    case (FApp1\<^sub>k s' sr)
+    with ev\<^sub>d_app1 obtain t'' where "(s' :\<^sub>k t' \<rightarrow> t'') \<and> (FApp1\<^sub>k e\<^sub>2 # sr :\<^sub>k t'' \<rightarrow> t)" by fastforce
+    with ev\<^sub>d_app1 FApp1\<^sub>k obtain b' ss' e'' where S': "iter (\<leadsto>\<^sub>k) (S\<^sub>k b s' e) (S\<^sub>k b' ss' e'') \<and> 
+      e\<^sub>1' = unstack' ss' e''" by metis
+    hence X: "iter (\<leadsto>\<^sub>k) (S\<^sub>k b (s' @ FApp1\<^sub>k e\<^sub>2 # sr) e) (S\<^sub>k b' (ss' @ FApp1\<^sub>k e\<^sub>2 # sr) e'')" by simp
+    from FApp1\<^sub>k S' have "App\<^sub>d e\<^sub>1' e\<^sub>2 = unstack' (ss' @ FApp1\<^sub>k e\<^sub>2 # sr) e''" by simp
+    with FApp1\<^sub>k X show ?case by blast
+  next
+    case (FApp2\<^sub>k s' sr)
+    hence "s = s' @ FApp2\<^sub>k e\<^sub>1 # sr \<and> e\<^sub>2 = unstack' s' e" by simp
+    with ev\<^sub>d_app1 obtain t\<^sub>1 where "(s' :\<^sub>k t' \<rightarrow> t\<^sub>1) \<and> (FApp2\<^sub>k e\<^sub>1 # sr :\<^sub>k t\<^sub>1 \<rightarrow> t)" by fastforce
+    with FApp2\<^sub>k have "([] \<turnstile>\<^sub>d e\<^sub>1 : Arrow t\<^sub>1 t) \<and> value\<^sub>d e\<^sub>1" by fastforce
+    with ev\<^sub>d_app1 show ?case by (metis val_no_eval\<^sub>d)
   qed
 next
   case (ev\<^sub>d_app2 e\<^sub>1 e\<^sub>2 e\<^sub>2')
-  thus ?case
-  proof (cases "all_returns s \<and> e = App\<^sub>d e\<^sub>1 e\<^sub>2")
-    case True
+  from ev\<^sub>d_app2(4) show ?case
+  proof (induction rule: unstack_to_app)
+    case Empty
     with ev\<^sub>d_app2 have B: "\<not>b" by (cases b) simp_all
-    from ev\<^sub>d_app2 True obtain t\<^sub>1 where T: "([] \<turnstile>\<^sub>d e\<^sub>1 : Arrow t\<^sub>1 tt) \<and> ([] \<turnstile>\<^sub>d e\<^sub>2 : t\<^sub>1)" by blast
+    from ev\<^sub>d_app2 Empty obtain t\<^sub>1 where T: "([] \<turnstile>\<^sub>d e\<^sub>1 : Arrow t\<^sub>1 tt) \<and> ([] \<turnstile>\<^sub>d e\<^sub>2 : t\<^sub>1)" by blast
     with ev\<^sub>d_app2 B obtain b' s' e'' where E: "iter (\<leadsto>\<^sub>k) (S\<^sub>k False [] e\<^sub>2) (S\<^sub>k b' s' e'') \<and> 
-      e\<^sub>2' = unwind' s' e''" by (metis unwind'.simps(1) tcs\<^sub>k_nil)
+      e\<^sub>2' = unstack' s' e''" by (metis unstack'.simps(1) tcs\<^sub>k_nil)
     hence "iter (\<leadsto>\<^sub>k) (S\<^sub>k False (FApp2\<^sub>k e\<^sub>1 # s) e\<^sub>2) (S\<^sub>k b' (s' @ FApp2\<^sub>k e\<^sub>1 # s) e'')" 
       by (metis eval\<^sub>k_under_iter append_Nil)
     moreover have "S\<^sub>k False s (App\<^sub>d e\<^sub>1 e\<^sub>2) \<leadsto>\<^sub>k S\<^sub>k False (FApp1\<^sub>k e\<^sub>2 # s) e\<^sub>1" by simp
@@ -181,48 +153,41 @@ next
     moreover have "S\<^sub>k True (FApp1\<^sub>k e\<^sub>2 # s) e\<^sub>1 \<leadsto>\<^sub>k S\<^sub>k False (FApp2\<^sub>k e\<^sub>1 # s) e\<^sub>2" by simp
     ultimately have "iter (\<leadsto>\<^sub>k) (S\<^sub>k False s (App\<^sub>d e\<^sub>1 e\<^sub>2)) (S\<^sub>k b' (s' @ FApp2\<^sub>k e\<^sub>1 # s) e'')" 
       by (metis iter_step iter_append)
-    with True B E show ?thesis by fastforce
+    with Empty B E show ?case by fastforce
   next
-    case False
-    with ev\<^sub>d_app2 obtain s' sr where S: "all_returns sr \<and> 
-      ((s = s' @ FApp1\<^sub>k e\<^sub>2 # sr \<and> e\<^sub>1 = unwind' s' e) \<or> 
-        (s = s' @ FApp2\<^sub>k e\<^sub>1 # sr \<and> e\<^sub>2 = unwind' s' e))" by blast
-    thus ?thesis
-    proof (cases "s = s' @ FApp1\<^sub>k e\<^sub>2 # sr \<and> e\<^sub>1 = unwind' s' e")
-      case True
-      with ev\<^sub>d_app2 have S': "all_returns s' \<and> e = e\<^sub>1" by simp 
-      with ev\<^sub>d_app2 True S obtain t\<^sub>1 where T: "t' = Arrow t\<^sub>1 t \<and> [] \<turnstile>\<^sub>d e\<^sub>2 : t\<^sub>1" by blast
-      have X: "e\<^sub>2 = unwind' [] e\<^sub>2" by simp
-      have E: "[] :\<^sub>k t' \<rightarrow> t'" by simp
-      have "False \<Longrightarrow> value\<^sub>d e\<^sub>2" by simp
-      with ev\<^sub>d_app2 T X E obtain b'' s'' e'' where E: "iter (\<leadsto>\<^sub>k) (S\<^sub>k False [] e\<^sub>2) (S\<^sub>k b'' s'' e'') \<and> 
-        e\<^sub>2' = unwind' s'' e''" by blast
-      hence "iter (\<leadsto>\<^sub>k) (S\<^sub>k False (FApp2\<^sub>k e\<^sub>1 # sr) e\<^sub>2) (S\<^sub>k b'' (s'' @ FApp2\<^sub>k e\<^sub>1 # sr) e'')" 
-        using eval\<^sub>k_under_iter by fastforce
-      moreover from ev\<^sub>d_app2 have "S\<^sub>k True (FApp1\<^sub>k e\<^sub>2 # sr) e\<^sub>1 \<leadsto>\<^sub>k S\<^sub>k False (FApp2\<^sub>k e\<^sub>1 # sr) e\<^sub>2" by simp
-      moreover from ev\<^sub>d_app2 S' have "iter (\<leadsto>\<^sub>k) (S\<^sub>k True (s' @ FApp1\<^sub>k e\<^sub>2 # sr) e\<^sub>1) 
-        (S\<^sub>k True (FApp1\<^sub>k e\<^sub>2 # sr) e\<^sub>1)" by simp
-      moreover from ev\<^sub>d_app2 S' have "iter (\<leadsto>\<^sub>k) (S\<^sub>k b (s' @ FApp1\<^sub>k e\<^sub>2 # sr) e\<^sub>1) 
-        (S\<^sub>k True (s' @ FApp1\<^sub>k e\<^sub>2 # sr) e\<^sub>1)" by simp
-      ultimately have Y: "iter (\<leadsto>\<^sub>k) (S\<^sub>k b (s' @ FApp1\<^sub>k e\<^sub>2 # sr) e\<^sub>1) 
-        (S\<^sub>k b'' (s'' @ FApp2\<^sub>k e\<^sub>1 # sr) e'')" by (metis iter_step iter_append)
-      from S E have "App\<^sub>d e\<^sub>1 e\<^sub>2' = unwind' (s'' @ FApp2\<^sub>k e\<^sub>1 # sr) e''" by simp
-      with True S' Y show ?thesis by auto
-    next
-      case False
-      with S have S': "s = s' @ FApp2\<^sub>k e\<^sub>1 # sr \<and> e\<^sub>2 = unwind' s' e" by simp
-      with ev\<^sub>d_app2 obtain t\<^sub>1 where "(s' :\<^sub>k t' \<rightarrow> t\<^sub>1) \<and> (FApp2\<^sub>k e\<^sub>1 # sr :\<^sub>k t\<^sub>1 \<rightarrow> t)" by fastforce
-      with ev\<^sub>d_app2 S' obtain b'' s'' e'' where E: "iter (\<leadsto>\<^sub>k) (S\<^sub>k b s' e) (S\<^sub>k b'' s'' e'') \<and> 
-        e\<^sub>2' = unwind' s'' e''" by blast
-      hence "iter (\<leadsto>\<^sub>k) (S\<^sub>k b (s' @ FApp2\<^sub>k e\<^sub>1 # sr) e) (S\<^sub>k b'' (s'' @ FApp2\<^sub>k e\<^sub>1 # sr) e'')" by simp
-      with S S' E show ?thesis by fastforce
-    qed
+    case (FApp1\<^sub>k s' sr)
+    with ev\<^sub>d_app2 have S': "all_returns s' \<and> e = e\<^sub>1" by simp 
+    with ev\<^sub>d_app2 FApp1\<^sub>k obtain t\<^sub>1 where T: "t' = Arrow t\<^sub>1 t \<and> [] \<turnstile>\<^sub>d e\<^sub>2 : t\<^sub>1" by blast
+    have X: "e\<^sub>2 = unstack' [] e\<^sub>2" by simp
+    have E: "[] :\<^sub>k t' \<rightarrow> t'" by simp
+    have "False \<Longrightarrow> value\<^sub>d e\<^sub>2" by simp
+    with ev\<^sub>d_app2 T X E obtain b'' s'' e'' where E: "iter (\<leadsto>\<^sub>k) (S\<^sub>k False [] e\<^sub>2) (S\<^sub>k b'' s'' e'') \<and> 
+      e\<^sub>2' = unstack' s'' e''" by blast
+    hence "iter (\<leadsto>\<^sub>k) (S\<^sub>k False (FApp2\<^sub>k e\<^sub>1 # sr) e\<^sub>2) (S\<^sub>k b'' (s'' @ FApp2\<^sub>k e\<^sub>1 # sr) e'')" 
+      using eval\<^sub>k_under_iter by fastforce
+    moreover from ev\<^sub>d_app2 have "S\<^sub>k True (FApp1\<^sub>k e\<^sub>2 # sr) e\<^sub>1 \<leadsto>\<^sub>k S\<^sub>k False (FApp2\<^sub>k e\<^sub>1 # sr) e\<^sub>2" by simp
+    moreover from ev\<^sub>d_app2 S' have "iter (\<leadsto>\<^sub>k) (S\<^sub>k True (s' @ FApp1\<^sub>k e\<^sub>2 # sr) e\<^sub>1) 
+      (S\<^sub>k True (FApp1\<^sub>k e\<^sub>2 # sr) e\<^sub>1)" by simp
+    moreover from ev\<^sub>d_app2 S' have "iter (\<leadsto>\<^sub>k) (S\<^sub>k b (s' @ FApp1\<^sub>k e\<^sub>2 # sr) e\<^sub>1) 
+      (S\<^sub>k True (s' @ FApp1\<^sub>k e\<^sub>2 # sr) e\<^sub>1)" by simp
+    ultimately have Y: "iter (\<leadsto>\<^sub>k) (S\<^sub>k b (s' @ FApp1\<^sub>k e\<^sub>2 # sr) e\<^sub>1) 
+      (S\<^sub>k b'' (s'' @ FApp2\<^sub>k e\<^sub>1 # sr) e'')" by (metis iter_step iter_append)
+    from FApp1\<^sub>k E have "App\<^sub>d e\<^sub>1 e\<^sub>2' = unstack' (s'' @ FApp2\<^sub>k e\<^sub>1 # sr) e''" by simp
+    with FApp1\<^sub>k S' Y show ?case by metis
+  next
+    case (FApp2\<^sub>k s' sr)
+    hence S': "s = s' @ FApp2\<^sub>k e\<^sub>1 # sr \<and> e\<^sub>2 = unstack' s' e" by simp
+    with ev\<^sub>d_app2 obtain t\<^sub>1 where "(s' :\<^sub>k t' \<rightarrow> t\<^sub>1) \<and> (FApp2\<^sub>k e\<^sub>1 # sr :\<^sub>k t\<^sub>1 \<rightarrow> t)" by fastforce
+    with ev\<^sub>d_app2 S' obtain b'' s'' e'' where E: "iter (\<leadsto>\<^sub>k) (S\<^sub>k b s' e) (S\<^sub>k b'' s'' e'') \<and> 
+      e\<^sub>2' = unstack' s'' e''" by blast
+    hence "iter (\<leadsto>\<^sub>k) (S\<^sub>k b (s' @ FApp2\<^sub>k e\<^sub>1 # sr) e) (S\<^sub>k b'' (s'' @ FApp2\<^sub>k e\<^sub>1 # sr) e'')" by simp
+    with FApp2\<^sub>k S' E show ?case by fastforce
   qed
 next
   case (ev\<^sub>d_app3 e\<^sub>2 t\<^sub>1 e\<^sub>1)
-  thus ?case
-  proof (cases "all_returns s \<and> e = App\<^sub>d (Lam\<^sub>d t\<^sub>1 e\<^sub>1) e\<^sub>2")
-    case True
+  from ev\<^sub>d_app3(2) show ?case
+  proof (induction rule: unstack_to_app)
+    case Empty
     with ev\<^sub>d_app3 have B: "\<not>b" by (cases b) simp_all
     have "S\<^sub>k False s (App\<^sub>d (Lam\<^sub>d t\<^sub>1 e\<^sub>1) e\<^sub>2) \<leadsto>\<^sub>k S\<^sub>k False (FApp1\<^sub>k e\<^sub>2 # s) (Lam\<^sub>d t\<^sub>1 e\<^sub>1)" by simp
     moreover have "S\<^sub>k False (FApp1\<^sub>k e\<^sub>2 # s) (Lam\<^sub>d t\<^sub>1 e\<^sub>1) \<leadsto>\<^sub>k S\<^sub>k True  (FApp1\<^sub>k e\<^sub>2 # s) (Lam\<^sub>d t\<^sub>1 e\<^sub>1)" 
@@ -235,80 +200,80 @@ next
       by simp
     ultimately have X: "iter (\<leadsto>\<^sub>k) (S\<^sub>k False s (App\<^sub>d (Lam\<^sub>d t\<^sub>1 e\<^sub>1) e\<^sub>2)) 
       (S\<^sub>k False (FReturn\<^sub>k # s) (subst\<^sub>d 0 e\<^sub>2 e\<^sub>1))" by (metis iter_step iter_refl iter_append)
-    from True have "subst\<^sub>d 0 e\<^sub>2 e\<^sub>1 = unwind' (FReturn\<^sub>k # s) (subst\<^sub>d 0 e\<^sub>2 e\<^sub>1)"
-      using unwind_returns by simp
-    with True B X show ?thesis by fastforce
+    from Empty have "subst\<^sub>d 0 e\<^sub>2 e\<^sub>1 = unstack' (FReturn\<^sub>k # s) (subst\<^sub>d 0 e\<^sub>2 e\<^sub>1)"
+      using unstack_returns by simp
+    with Empty B X show ?case by fastforce
   next
-    case False
-    with ev\<^sub>d_app3 obtain s' sr where S: "all_returns sr \<and> 
-      ((s = s' @ FApp1\<^sub>k e\<^sub>2 # sr \<and> Lam\<^sub>d t\<^sub>1 e\<^sub>1 = unwind' s' e) \<or> 
-        (s = s' @ FApp2\<^sub>k (Lam\<^sub>d t\<^sub>1 e\<^sub>1) # sr \<and> e\<^sub>2 = unwind' s' e))" by blast
-    thus ?thesis
-    proof (cases "s = s' @ FApp1\<^sub>k e\<^sub>2 # sr \<and> Lam\<^sub>d t\<^sub>1 e\<^sub>1 = unwind' s' e")
-      case True
-      moreover have "value\<^sub>d (Lam\<^sub>d t\<^sub>1 e\<^sub>1)" by simp
-      ultimately have S': "all_returns s' \<and> e = Lam\<^sub>d t\<^sub>1 e\<^sub>1" by simp
-      have "S\<^sub>k True (FApp1\<^sub>k e\<^sub>2 # sr) (Lam\<^sub>d t\<^sub>1 e\<^sub>1) \<leadsto>\<^sub>k S\<^sub>k False (FApp2\<^sub>k (Lam\<^sub>d t\<^sub>1 e\<^sub>1) # sr) e\<^sub>2" by simp
-      moreover from ev\<^sub>d_app3 have "iter (\<leadsto>\<^sub>k) (S\<^sub>k False (FApp2\<^sub>k (Lam\<^sub>d t\<^sub>1 e\<^sub>1) # sr) e\<^sub>2) 
-        (S\<^sub>k True (FApp2\<^sub>k (Lam\<^sub>d t\<^sub>1 e\<^sub>1) # sr) e\<^sub>2)" by simp
-      moreover from ev\<^sub>d_app3 have "S\<^sub>k True (FApp2\<^sub>k (Lam\<^sub>d t\<^sub>1 e\<^sub>1) # sr) e\<^sub>2 \<leadsto>\<^sub>k 
-        S\<^sub>k False (FReturn\<^sub>k # sr) (subst\<^sub>d 0 e\<^sub>2 e\<^sub>1)" by simp
-      moreover from S' have "iter (\<leadsto>\<^sub>k) (S\<^sub>k True (s' @ FApp1\<^sub>k e\<^sub>2 # sr) (Lam\<^sub>d t\<^sub>1 e\<^sub>1)) 
-        (S\<^sub>k True (FApp1\<^sub>k e\<^sub>2 # sr) (Lam\<^sub>d t\<^sub>1 e\<^sub>1))" by simp
-      moreover have "iter (\<leadsto>\<^sub>k) (S\<^sub>k b (s' @ FApp1\<^sub>k e\<^sub>2 # sr) (Lam\<^sub>d t\<^sub>1 e\<^sub>1)) 
-        (S\<^sub>k True (s' @ FApp1\<^sub>k e\<^sub>2 # sr) (Lam\<^sub>d t\<^sub>1 e\<^sub>1))" by simp
-      ultimately have X: "iter (\<leadsto>\<^sub>k) (S\<^sub>k b (s' @ FApp1\<^sub>k e\<^sub>2 # sr) (Lam\<^sub>d t\<^sub>1 e\<^sub>1)) 
-        (S\<^sub>k False (FReturn\<^sub>k # sr) (subst\<^sub>d 0 e\<^sub>2 e\<^sub>1))" by (metis iter_step iter_refl iter_append)
-      from S True have "subst\<^sub>d 0 e\<^sub>2 e\<^sub>1 = unwind' (FReturn\<^sub>k # sr) (subst\<^sub>d 0 e\<^sub>2 e\<^sub>1)" 
-        using unwind_returns by simp
-      with True S' X show ?thesis by fastforce
-    next
-      case False
-      with S ev\<^sub>d_app3 have S': "all_returns s' \<and> e = e\<^sub>2" by simp
-      from ev\<^sub>d_app3 have "S\<^sub>k True (FApp2\<^sub>k (Lam\<^sub>d t\<^sub>1 e\<^sub>1) # sr) e\<^sub>2 \<leadsto>\<^sub>k 
-        S\<^sub>k False (FReturn\<^sub>k # sr) (subst\<^sub>d 0 e\<^sub>2 e\<^sub>1)" by simp
-      hence "iter (\<leadsto>\<^sub>k) (S\<^sub>k True (FApp2\<^sub>k (Lam\<^sub>d t\<^sub>1 e\<^sub>1) # sr) e\<^sub>2) 
-        (S\<^sub>k False (FReturn\<^sub>k # sr) (subst\<^sub>d 0 e\<^sub>2 e\<^sub>1))" by (metis iter_step iter_refl)
-      moreover from ev\<^sub>d_app3 S' have "iter (\<leadsto>\<^sub>k) (S\<^sub>k True (s' @ FApp2\<^sub>k (Lam\<^sub>d t\<^sub>1 e\<^sub>1) # sr) e\<^sub>2) 
-        (S\<^sub>k True (FApp2\<^sub>k (Lam\<^sub>d t\<^sub>1 e\<^sub>1) # sr) e\<^sub>2)" by simp
-      moreover from ev\<^sub>d_app3 have "iter (\<leadsto>\<^sub>k) (S\<^sub>k b (s' @ FApp2\<^sub>k (Lam\<^sub>d t\<^sub>1 e\<^sub>1) # sr) e\<^sub>2) 
-        (S\<^sub>k True (s' @ FApp2\<^sub>k (Lam\<^sub>d t\<^sub>1 e\<^sub>1) # sr) e\<^sub>2)" by simp
-      ultimately have X: "iter (\<leadsto>\<^sub>k) (S\<^sub>k b (s' @ FApp2\<^sub>k (Lam\<^sub>d t\<^sub>1 e\<^sub>1) # sr) e\<^sub>2) 
-        (S\<^sub>k False (FReturn\<^sub>k # sr) (subst\<^sub>d 0 e\<^sub>2 e\<^sub>1))" by (metis iter_append)
-      from S have "subst\<^sub>d 0 e\<^sub>2 e\<^sub>1 = unwind' (FReturn\<^sub>k # sr) (subst\<^sub>d 0 e\<^sub>2 e\<^sub>1)" 
-        using unwind_returns by simp
-      with S False S' X show ?thesis by metis
-    qed
+    case (FApp1\<^sub>k s' sr)
+    moreover have "value\<^sub>d (Lam\<^sub>d t\<^sub>1 e\<^sub>1)" by simp
+    ultimately have S': "all_returns s' \<and> e = Lam\<^sub>d t\<^sub>1 e\<^sub>1" by simp
+    have "S\<^sub>k True (FApp1\<^sub>k e\<^sub>2 # sr) (Lam\<^sub>d t\<^sub>1 e\<^sub>1) \<leadsto>\<^sub>k S\<^sub>k False (FApp2\<^sub>k (Lam\<^sub>d t\<^sub>1 e\<^sub>1) # sr) e\<^sub>2" by simp
+    moreover from ev\<^sub>d_app3 have "iter (\<leadsto>\<^sub>k) (S\<^sub>k False (FApp2\<^sub>k (Lam\<^sub>d t\<^sub>1 e\<^sub>1) # sr) e\<^sub>2) 
+      (S\<^sub>k True (FApp2\<^sub>k (Lam\<^sub>d t\<^sub>1 e\<^sub>1) # sr) e\<^sub>2)" by simp
+    moreover from ev\<^sub>d_app3 have "S\<^sub>k True (FApp2\<^sub>k (Lam\<^sub>d t\<^sub>1 e\<^sub>1) # sr) e\<^sub>2 \<leadsto>\<^sub>k 
+      S\<^sub>k False (FReturn\<^sub>k # sr) (subst\<^sub>d 0 e\<^sub>2 e\<^sub>1)" by simp
+    moreover from S' have "iter (\<leadsto>\<^sub>k) (S\<^sub>k True (s' @ FApp1\<^sub>k e\<^sub>2 # sr) (Lam\<^sub>d t\<^sub>1 e\<^sub>1)) 
+      (S\<^sub>k True (FApp1\<^sub>k e\<^sub>2 # sr) (Lam\<^sub>d t\<^sub>1 e\<^sub>1))" by simp
+    moreover have "iter (\<leadsto>\<^sub>k) (S\<^sub>k b (s' @ FApp1\<^sub>k e\<^sub>2 # sr) (Lam\<^sub>d t\<^sub>1 e\<^sub>1)) 
+      (S\<^sub>k True (s' @ FApp1\<^sub>k e\<^sub>2 # sr) (Lam\<^sub>d t\<^sub>1 e\<^sub>1))" by simp
+    ultimately have X: "iter (\<leadsto>\<^sub>k) (S\<^sub>k b (s' @ FApp1\<^sub>k e\<^sub>2 # sr) (Lam\<^sub>d t\<^sub>1 e\<^sub>1)) 
+      (S\<^sub>k False (FReturn\<^sub>k # sr) (subst\<^sub>d 0 e\<^sub>2 e\<^sub>1))" by (metis iter_step iter_refl iter_append)
+    from FApp1\<^sub>k have "subst\<^sub>d 0 e\<^sub>2 e\<^sub>1 = unstack' (FReturn\<^sub>k # sr) (subst\<^sub>d 0 e\<^sub>2 e\<^sub>1)" 
+      using unstack_returns by simp
+    with FApp1\<^sub>k S' X show ?case by fastforce
+  next
+    case (FApp2\<^sub>k s' sr)
+    with ev\<^sub>d_app3 have S': "all_returns s' \<and> e = e\<^sub>2" by simp
+    from ev\<^sub>d_app3 have "S\<^sub>k True (FApp2\<^sub>k (Lam\<^sub>d t\<^sub>1 e\<^sub>1) # sr) e\<^sub>2 \<leadsto>\<^sub>k 
+      S\<^sub>k False (FReturn\<^sub>k # sr) (subst\<^sub>d 0 e\<^sub>2 e\<^sub>1)" by simp
+    hence "iter (\<leadsto>\<^sub>k) (S\<^sub>k True (FApp2\<^sub>k (Lam\<^sub>d t\<^sub>1 e\<^sub>1) # sr) e\<^sub>2) 
+      (S\<^sub>k False (FReturn\<^sub>k # sr) (subst\<^sub>d 0 e\<^sub>2 e\<^sub>1))" by (metis iter_step iter_refl)
+    moreover from ev\<^sub>d_app3 S' have "iter (\<leadsto>\<^sub>k) (S\<^sub>k True (s' @ FApp2\<^sub>k (Lam\<^sub>d t\<^sub>1 e\<^sub>1) # sr) e\<^sub>2) 
+      (S\<^sub>k True (FApp2\<^sub>k (Lam\<^sub>d t\<^sub>1 e\<^sub>1) # sr) e\<^sub>2)" by simp
+    moreover from ev\<^sub>d_app3 have "iter (\<leadsto>\<^sub>k) (S\<^sub>k b (s' @ FApp2\<^sub>k (Lam\<^sub>d t\<^sub>1 e\<^sub>1) # sr) e\<^sub>2) 
+      (S\<^sub>k True (s' @ FApp2\<^sub>k (Lam\<^sub>d t\<^sub>1 e\<^sub>1) # sr) e\<^sub>2)" by simp
+    ultimately have X: "iter (\<leadsto>\<^sub>k) (S\<^sub>k b (s' @ FApp2\<^sub>k (Lam\<^sub>d t\<^sub>1 e\<^sub>1) # sr) e\<^sub>2) 
+      (S\<^sub>k False (FReturn\<^sub>k # sr) (subst\<^sub>d 0 e\<^sub>2 e\<^sub>1))" by (metis iter_append)
+    from FApp2\<^sub>k have "subst\<^sub>d 0 e\<^sub>2 e\<^sub>1 = unstack' (FReturn\<^sub>k # sr) (subst\<^sub>d 0 e\<^sub>2 e\<^sub>1)" 
+      using unstack_returns by simp
+    with FApp2\<^sub>k S' X show ?case by metis
   qed
 qed
 
-theorem completed [simp]: "\<Sigma> :\<^sub>k t \<Longrightarrow> unwind \<Sigma> \<leadsto>\<^sub>d e' \<Longrightarrow> \<exists>\<Sigma>'. iter (\<leadsto>\<^sub>k) \<Sigma> \<Sigma>' \<and> e' = unwind \<Sigma>'"
-proof (induction \<Sigma> t rule: typing_state\<^sub>k.induct)
+text \<open>Correctness is now simple to state and prove. We also extend the theorem to cover full
+evaluation from an initial state to a final one.\<close>
+
+theorem correct\<^sub>k [simp]: "\<Sigma>\<^sub>k :\<^sub>k t \<Longrightarrow> unstack \<Sigma>\<^sub>k \<leadsto>\<^sub>d e' \<Longrightarrow> 
+  \<exists>\<Sigma>\<^sub>k'. iter (\<leadsto>\<^sub>k) \<Sigma>\<^sub>k \<Sigma>\<^sub>k' \<and> e' = unstack \<Sigma>\<^sub>k'"
+proof (induction \<Sigma>\<^sub>k t rule: typing_state\<^sub>k.induct)
   case (tc_state\<^sub>k s t' t e b)
-  then obtain b' s' e'' where "iter (\<leadsto>\<^sub>k) (S\<^sub>k b s e) (S\<^sub>k b' s' e'') \<and> e' = unwind' s' e''" by fastforce
+  then obtain b' s' e'' where "iter (\<leadsto>\<^sub>k) (S\<^sub>k b s e) (S\<^sub>k b' s' e'') \<and> e' = unstack' s' e''" 
+    by fastforce
   thus ?case by fastforce
 qed
 
-lemma [simp]: "iter (\<leadsto>\<^sub>d) (unwind \<Sigma>) e' \<Longrightarrow> \<Sigma> :\<^sub>k t \<Longrightarrow> \<exists>\<Sigma>'. iter (\<leadsto>\<^sub>k) \<Sigma> \<Sigma>' \<and> e' = unwind \<Sigma>'"
-proof (induction "unwind \<Sigma>" e' arbitrary: \<Sigma> rule: iter.induct)
+lemma correct\<^sub>k_iter [simp]: "iter (\<leadsto>\<^sub>d) (unstack \<Sigma>\<^sub>k) e' \<Longrightarrow> \<Sigma>\<^sub>k :\<^sub>k t \<Longrightarrow> 
+  \<exists>\<Sigma>\<^sub>k'. iter (\<leadsto>\<^sub>k) \<Sigma>\<^sub>k \<Sigma>\<^sub>k' \<and> e' = unstack \<Sigma>\<^sub>k'"
+proof (induction "unstack \<Sigma>\<^sub>k" e' arbitrary: \<Sigma>\<^sub>k rule: iter.induct)
   case (iter_step e' e'')
-  moreover then obtain \<Sigma>' where S: "iter (\<leadsto>\<^sub>k) \<Sigma> \<Sigma>' \<and> e' = unwind \<Sigma>'" by fastforce
-  moreover with iter_step have "\<Sigma>' :\<^sub>k t" by fastforce
-  ultimately obtain \<Sigma>'' where "iter (\<leadsto>\<^sub>k) \<Sigma>' \<Sigma>'' \<and> e'' = unwind \<Sigma>''" by fastforce
-  with S have "iter (\<leadsto>\<^sub>k) \<Sigma> \<Sigma>'' \<and> e'' = unwind \<Sigma>''" by (metis iter_append)
+  moreover then obtain \<Sigma>\<^sub>k' where S: "iter (\<leadsto>\<^sub>k) \<Sigma>\<^sub>k \<Sigma>\<^sub>k' \<and> e' = unstack \<Sigma>\<^sub>k'" by fastforce
+  moreover with iter_step have "\<Sigma>\<^sub>k' :\<^sub>k t" by fastforce
+  ultimately obtain \<Sigma>\<^sub>k'' where "iter (\<leadsto>\<^sub>k) \<Sigma>\<^sub>k' \<Sigma>\<^sub>k'' \<and> e'' = unstack \<Sigma>\<^sub>k''" by fastforce
+  with S have "iter (\<leadsto>\<^sub>k) \<Sigma>\<^sub>k \<Sigma>\<^sub>k'' \<and> e'' = unstack \<Sigma>\<^sub>k''" by (metis iter_append)
   then show ?case by fastforce
 qed force+
 
-lemma [simp]: "iter (\<leadsto>\<^sub>d) e v \<Longrightarrow> [] \<turnstile>\<^sub>d e : t \<Longrightarrow> value\<^sub>d v \<Longrightarrow> 
+lemma correct\<^sub>k_full_eval [simp]: "iter (\<leadsto>\<^sub>d) e v \<Longrightarrow> [] \<turnstile>\<^sub>d e : t \<Longrightarrow> value\<^sub>d v \<Longrightarrow> 
   iter (\<leadsto>\<^sub>k) (S\<^sub>k False [FReturn\<^sub>k] e) (S\<^sub>k True [] v)"
 proof -
   assume "[] \<turnstile>\<^sub>d e : t"
   hence "S\<^sub>k False [FReturn\<^sub>k] e :\<^sub>k t" by (metis tcs\<^sub>k_nil tcs\<^sub>k_cons_ret tc_state\<^sub>k)
   moreover assume "iter (\<leadsto>\<^sub>d) e v"
-  ultimately obtain \<Sigma>' where S: "iter (\<leadsto>\<^sub>k) (S\<^sub>k False [FReturn\<^sub>k] e) \<Sigma>' \<and> v = unwind \<Sigma>'" by fastforce
+  ultimately obtain \<Sigma>\<^sub>k' where S: "iter (\<leadsto>\<^sub>k) (S\<^sub>k False [FReturn\<^sub>k] e) \<Sigma>\<^sub>k' \<and> v = unstack \<Sigma>\<^sub>k'" 
+    by fastforce
   moreover assume V: "value\<^sub>d v"
-  ultimately obtain b sr where "\<Sigma>' = S\<^sub>k b (sr @ []) v \<and> all_returns sr" by fastforce
-  moreover with V have "iter (\<leadsto>\<^sub>k) \<Sigma>' (S\<^sub>k True [] v)" by (metis eval_returns)
+  ultimately obtain b sr where "\<Sigma>\<^sub>k' = S\<^sub>k b (sr @ []) v \<and> all_returns sr" by fastforce
+  moreover with V have "iter (\<leadsto>\<^sub>k) \<Sigma>\<^sub>k' (S\<^sub>k True [] v)" by (metis eval_returns_in_front)
   with S show "iter (\<leadsto>\<^sub>k) (S\<^sub>k False [FReturn\<^sub>k] e) (S\<^sub>k True [] v)" by (metis iter_append)
 qed
 
